Flapjack.lean
@@ -44,6 +44,7 @@ import Flapjack.Word
 import Flapjack.Stack
 import Flapjack.StackAlloc
 import Flapjack.StackAlloc.Runtime
+import Flapjack.StackAlloc.Machine
 import Flapjack.StackRemove
 import Flapjack.Lab
 import Flapjack.RiscV.Lab
